

→ reverse algorithm

→ [1, 2, 3, 4, 5]
 $\begin{matrix} 1 & 2 & 3 & 4 & 5 \\ i & j & & & \end{matrix}$

→ [5, 4, 3, 2, 1]
 $\begin{matrix} 5 & 4 & 3 & 2 & 1 \\ i & j & & & \end{matrix}$

$\begin{matrix} 6 & 5 & 4 & 3 & 2 & 1 \\ \hline i & j & & & & \end{matrix}$ = 6
 $\textcircled{5} = n-1$
 $i = 0, j = n-1$

$(i < j)$
 $(i \neq j)$

[1, 2, 3, 4, 5, 6]
 $\begin{matrix} 1 & 2 & 3 & 4 & 5 & 6 \\ i & & & & & j \end{matrix}$

$i = 0$
 $j = n-1$

while $(i < j)$ {
 $\text{temp} = \text{arr}[i]$
 $\text{arr}[i] = \text{arr}[j]$
 $\text{arr}[j] = \text{temp}$
 $i++$
 $j--$
 }

$\{ \rightarrow \textcircled{n^2} \quad n^3$
 $\{ \rightarrow \textcircled{7} \quad 3, 1 \}$

3

$[1, 2, 3, 4, 5, 6, 7]$
 $[5, 6, 7, 1, 2, 3, 4]$

$k = 3$

$= n - k$

$j < \underline{k}$

$[1, 2, 3, 4, 5, 6, 7]$

$k = \underline{2}$

$k = k \% 2 \dots 1$

~~$\text{reverse}(arr, 0, n-1)$~~
 $(k-1)$
 $(n-1)$